#+title: Fundamental polynomials of Lagrange
#+roam_alias: "Fundamental polynomials of Lagrange"
#+roam_tags: "Numeric Methods" "Definition" "Polynomials" "Lagrange"

* Fundamental polynomials of Lagrange
$l_{k,n}(x_i) = \delta_{ki}$ ([[file:Kronecker Delta.org][Kronecker Delta)]]

* Solved Problems

** Problem 1

Let $l_{k,n}(x_i)$, $k\in\overline{0,n}$ are the Fundamental polynomials of
Lagrange for the knots $x_0, \dots, x_n$

Then $\sum_{k=0}^{n}l_{kn}(x) = 1, \forall{}x$

*** Solution

Let $f(x) = 1$

f(x) \in \pi_n \Rightarrow f(x) \equiv L_n(f;x) \equiv 1         }
                                       } \Rightarrow \sum_{k=0}^{n}l_{nk}(x) = L_n(f;x) = 1
L_{n}(f;x) = \sum_{k=0}^{n}f(x_k)l_{kn}(x) = \sum_{k=0}^{n}1*l_{kn}(x)  }

** Problem 2
Prove that $\sum_{k=0}^{n}x_k^{m}l_{kn}(x) = x^{m}$, $m=\overline{0,n}$

*** Solution

Let $f(x) = x^m$, $m = \overline{0,n}$

f(x) \in \pi_n, m = \overline{0,n} \Rightarrow (x) \equiv L_n(f;x) = x^m, $m = \overline{0,n}$
                                            } \Rightarrow L_n(f;x) = \sum_{k=0}^{n}x_k^{m}l_{kn}(x) = x^m, $m = \overline{0,n}$
L_n(f;x) = \sum_{k=0}^{n}f(x_k)l_{kn}(x) = \sum_{k=0}^{n}x_k^{m}l_{kn}(x)
