#+title: Lagrange Interpolation Problem
#+startup: latexpreview
#+roam_alias: "Lagrange Interpolation Problem"
#+roam_tags: "Lagrange" "Interpolation" "Definition" "Numeric Methods"

* Lagrange Interpolation Problem
Let $x_0, ..., x_n$ such that $x_i \ne x_j$, $i \ne h$ - Knots of interpolation.
Let $y_0, ..., y_n$ be values.
Find $(1)$ $p(x_i) = y_i$,  $i = \overline{0,n}$
** Unique
:PROPERTIES:
:ID:       528f5e8b-6a96-44c8-86c7-3635791b7c59
:END:

Let's assume $\exists{}u,v \in \pi_{n}$ solve $(1)$, i.e $u(x_i)=v(x_{i})=y_{i}$, $i=\overline{0,n}$.


Let $p(x) = u(x) - v(x)$, $p \in \pi_{n}$.

Then $p(x_{i}) = u(x_{i}) - v(x_{i}) = y_{i} - y_{i} = 0$, $i = \overline{0,n}$

and therefore $p \in \pi_{n}$ has $n+1$ different zeroes: $x_{0}, .., x_{n}$.


As a consequence from the [[file:fundamental_theorem_of_algebra.org][Fundamental Theorem of Algebra]]
we know that $p(x) \equiv 0$, i.e $u(x) \equiv v(x)$. $\square$
q
** Existence

We will construct the solution to the Lagrange Interpolation Problem.

Let $p(x) = \sum_{k=0}^{n}\limits{}y_{k}l_{k,n}(x)$ where $l_{k,n}(x) \in \pi_{n}$ $(2)$

Let $l_{k,n}(x_i)$ - [[file:fundamental_polynomials_of_lagrange.org][Fundamental polynomials of Lagrange]]
$(3)$

If we know $l_{k,n}(x)$, k=$i = \overline{0,n}$
then p(x) is the solution to the Lagrange Interpolation Problem:

\[p(x_i) =_{(2)}\sum_{k=0}^{n}y_{k}l_{k,n}(x_i) =^{(3)}\sum_{k=0}^{n}y_{k}\delta_{ki}(x_i) = y_i\], $i = \overline{0,n}$

\Rightarrow $p(x)$ is a solution to Lagrange Interpolation Problem
also known as [[file:formula_of_lagrange_for_interpolation.org][Formula of Lagrange for Interpolation]].

*** Constructing $l_k,n(x)$
Let $l_{k,n}(x) \in \pi_{n}$ and $l_{k,n}$ has $n$ different zeroes:
$x_{0}, \dots, x_{k-1}, x_{k+1}, \dots, x_{n}$ (due to $(3)$, defined via [[file:kronecker_delta.org][Kronecker Delta]])


Then:

\[l_{k,n}(x) = A(x-x_{0})\dots(x-x_{k-1})(x-x_{k+1})\dots(x-x_{n}) \Rightarrow A = \frac{1}{\prod_{i=0,i\neq{}k}^{n}\limits{}(x_{k}-x_{i})}\]

Finally:

$(4)$ \[l_k,n(x) = \frac{(x-x_0)\dots(x-x_{k-1})(x-x_{k+1})\dots(x-x_n)}{(x_k-x_0)\dots(x_k-x_{k-1})(x_k-x_{k+1})\dots(x_k-x_n)} = \prod_{i=0,i\neq{}k}^{n}\limits{}\frac{x-x_{i}}{(x_{k}-x_{i})}\square\]
